Kura/Graph/Edges.lean
@@ -4,55 +4,57 @@ import Kura.Dep.Finset
 import Kura.Dep.Option
 
 
+open Sym2
+
 -- Do I need a separate none (edge not bound) that is not dir (none × none)?
 -- For now, dir (none × none) represents that the edge is not bound
-inductive edge (V : Type*) [LinearOrder V]
+inductive edge (V : Type*)
 | dir : Option V × Option V → edge V
 | undir : Sym2 V → edge V
 deriving Inhabited
 
 -- def edge (V : Type*) [DecidableEq V] := Option V × Option V ⊕ Sym2 V
 
-unsafe instance [Repr V] [LinearOrder V] : Repr (edge V) where
+unsafe instance [Repr V] : Repr (edge V) where
   reprPrec e _ := match e with
     | edge.dir (a, b) => repr a ++ "-→" ++ repr b
     | edge.undir s => repr s
 
 namespace edge
 
-variable {V : Type*} [LinearOrder V] (e : edge V)
+variable {V : Type*} (e : edge V)
 
 instance instNonempty [Nonempty V] : Nonempty (edge V) :=
   Nonempty.intro (undir s(Classical.ofNonempty, Classical.ofNonempty))
 
-def isDir  : Bool := match e with
+def isDir  : Prop := match e with
   | dir _ => true
   | _ => false
 
-def isUndir : Bool := match e with
+def isUndir : Prop := match e with
   | undir _ => true
   | _ => false
 
-def isFull : Bool := match e with
+def isFull : Prop := match e with
   | dir (some _, some _) => true
   | undir _ => true
   | _ => false
 
-def isHalf : Bool := match e with
+def isHalf : Prop := match e with
   | dir (some _, none) => true
   | dir (none, some _) => true
   | _ => false
 
-def isFree : Bool := match e with
+def isFree : Prop := match e with
   | dir (none, none) => true
   | _ => false
 
-def isLoop : Bool := match e with
+def isLoop : Prop := match e with
   | dir (some a, some b) => a = b
   | undir s => s.IsDiag
   | _ => false
 
-def isArc : Bool := match e with
+def isArc : Prop := match e with
   | dir (some a, some b) => a ≠ b
   | _ => false
 
@@ -119,7 +121,7 @@ lemma undir_isLoop_iff (s : Sym2 V) : isLoop (undir s) ↔ s.IsDiag := by
 
 @[simp high]
 lemma undir_isLoop_iff' (a b : V) : isLoop (undir s(a, b)) ↔ a = b := by
-  rw [undir_isLoop_iff, Sym2.isDiag_iff_proj_eq]
+  rw [undir_isLoop_iff, isDiag_iff_proj_eq]
 
 @[simp]
 lemma dir_isFull_iff (a b : Option V) : isFull (dir (a, b)) ↔ a.isSome ∧ b.isSome := by
@@ -159,7 +161,7 @@ lemma undir_endAt (s : Sym2 V) : (undir s).endAt = s.toMultiset := by rfl
 instance instedgeMem : Membership V (edge V) where
   mem e v := v ∈ e.endAt
 
-instance instMemDecPred : ∀ (u : V), Decidable (u ∈ e) := by
+instance instMemDecPred [DecidableEq V] : ∀ (u : V), Decidable (u ∈ e) := by
   cases e <;> simp only [instedgeMem] <;> infer_instance
 
 lemma mem_endAt_iff_mem (e : edge V) (v : V) : v ∈ e.endAt ↔ v ∈ e := by rfl
@@ -177,12 +179,12 @@ lemma mem_dir_some_snd (a : Option V) (b : V) : b ∈ dir (a, some b) := by
 
 lemma mem_toMultiset_of_undir (e : Sym2 V) (v : V) : v ∈ undir e ↔ v ∈ e.toMultiset := by
   simp only [instedgeMem, endAt, Multiset.insert_eq_cons, Multiset.empty_eq_zero, List.foldl_cons,
-    Multiset.cons_zero, List.foldl_nil, Sym2.mem_toMultiset_iff]
+    Multiset.cons_zero, List.foldl_nil, mem_toMultiset_iff]
 
 @[simp]
 lemma mem_undir_iff (e : Sym2 V) (v : V) : v ∈ undir e ↔ v ∈ e := by
   simp only [instedgeMem, endAt, Multiset.insert_eq_cons, Multiset.empty_eq_zero, List.foldl_cons,
-    Multiset.cons_zero, List.foldl_nil, Sym2.mem_toMultiset_iff]
+    Multiset.cons_zero, List.foldl_nil, mem_toMultiset_iff]
 
 def startAt : Multiset V := match e with
   | dir (a, _) =>
@@ -202,11 +204,11 @@ lemma undir_startAt (s : Sym2 V) : (undir s).startAt = s.toMultiset := by rfl
 
 @[simp]
 lemma mem_startAt_undir (s : Sym2 V) (v : V) : v ∈ startAt (undir s) ↔ v ∈ s := by
-  simp only [startAt, Sym2.mem_toMultiset_iff]
+  simp only [startAt, mem_toMultiset_iff]
 
 @[simp]
 lemma undir_startAt_card (s : Sym2 V) : Multiset.card (undir s).startAt = 2 := by
-  simp only [startAt, Sym2.toMultiset_card]
+  simp only [startAt, toMultiset_card]
 
 lemma dir_startAt_card (x : Option V × Option V) : Multiset.card (dir x : edge V).startAt < 2 := by
   obtain ⟨a, b⟩ := x
@@ -230,7 +232,7 @@ lemma startAt_subset_endAt (e : edge V) : e.startAt ⊆ e.endAt := by
       Multiset.insert_eq_cons, Multiset.empty_eq_zero, List.foldl_cons, Multiset.cons_zero,
       List.foldl_nil, Multiset.mem_cons, true_or, Multiset.not_mem_zero]
   | undir s =>
-    simp_all only [undir_startAt, Sym2.mem_toMultiset_iff, undir_endAt]
+    simp_all only [undir_startAt, mem_toMultiset_iff, undir_endAt]
 
 lemma mem_of_mem_startAt : ∀ v, v ∈ e.startAt → v ∈ e := by
   unfold instedgeMem
@@ -254,11 +256,11 @@ lemma undir_finishAt (s : Sym2 V) : (undir s).finishAt = s.toMultiset := by rfl
 
 @[simp]
 lemma mem_finishAt_undir (s : Sym2 V) (v : V) : v ∈ finishAt (undir s) ↔ v ∈ s := by
-  simp only [finishAt, Sym2.mem_toMultiset_iff]
+  simp only [finishAt, mem_toMultiset_iff]
 
 @[simp]
 lemma undir_finishAt_card (s : Sym2 V) : Multiset.card (undir s).finishAt = 2 := by
-  simp only [finishAt, Sym2.toMultiset_card]
+  simp only [finishAt, toMultiset_card]
 
 @[simp]
 lemma dir_finishAt_card (x : Option V × Option V) : Multiset.card (dir x : edge V).finishAt < 2 := by
@@ -282,14 +284,15 @@ lemma finishAt_subset_endAt (e : edge V) : e.finishAt ⊆ e.endAt := by
       Multiset.insert_eq_cons, Multiset.empty_eq_zero, List.foldl_cons, Multiset.cons_zero,
       List.foldl_nil, Multiset.mem_cons, or_true, Multiset.not_mem_zero]
   | undir s =>
-    simp_all only [undir_finishAt, Sym2.mem_toMultiset_iff, undir_endAt]
+    simp_all only [undir_finishAt, mem_toMultiset_iff, undir_endAt]
 
 lemma mem_of_mem_finishAt : ∀ v, v ∈ e.finishAt → v ∈ e := by
   unfold instedgeMem
   exact finishAt_subset_endAt e
 
 @[simp]
-lemma startAt_finishAt_not_disjoint_of_isLoop (e : edge V) : e.isLoop → e.startAt ∩ e.finishAt ≠ ∅ := by
+lemma startAt_finishAt_not_disjoint_of_isLoop [DecidableEq V] (e : edge V) :
+    e.isLoop → e.startAt ∩ e.finishAt ≠ ∅ := by
   intro hloop
   match e with
   | dir (some a, some b) =>
@@ -299,7 +302,7 @@ lemma startAt_finishAt_not_disjoint_of_isLoop (e : edge V) : e.isLoop → e.star
       Multiset.singleton_ne_zero, not_false_eq_true]
   | undir s =>
     simp only [startAt, finishAt, Multiset.inter_self, Multiset.empty_eq_zero, ne_eq, ←
-      Multiset.card_eq_zero, Sym2.toMultiset_card, OfNat.ofNat_ne_zero, not_false_eq_true]
+      Multiset.card_eq_zero, toMultiset_card, OfNat.ofNat_ne_zero, not_false_eq_true]
 
 @[ext]
 lemma ext (e e' : edge V) (hstart : e.startAt = e'.startAt) (hfin : e.finishAt = e'.finishAt) :
@@ -311,7 +314,7 @@ lemma ext (e e' : edge V) (hstart : e.startAt = e'.startAt) (hfin : e.finishAt =
   | undir s, undir s' =>
     simp_all only [undir_startAt, undir_finishAt, undir.injEq]
     ext v
-    rw [← Sym2.mem_toMultiset_iff, hstart, Sym2.mem_toMultiset_iff]
+    rw [← mem_toMultiset_iff, hstart, mem_toMultiset_iff]
   | dir (a, b), undir s =>
     exfalso
     apply dir_undir_finishAt_not_eq (a, b) s hfin
@@ -320,17 +323,17 @@ lemma ext (e e' : edge V) (hstart : e.startAt = e'.startAt) (hfin : e.finishAt =
     apply dir_undir_finishAt_not_eq (a, b) s hfin.symm
 
 
-def gofrom? (v : V) : Option V := match e with
+def gofrom? [DecidableEq V] (v : V) : Option V := match e with
   | dir (a, b) => if a = v then b else none
-  | undir s => if h : v ∈ s then (@Sym2.Mem.other' V _ v s h) else none
+  | undir s => if h : v ∈ s then (@Mem.other' V _ v s h) else none
 
-def goback? (v : V) : Option V := match e with
+def goback? [DecidableEq V] (v : V) : Option V := match e with
   | dir (a, b) => if b = v then a else none
-  | undir s => if h : v ∈ s then (@Sym2.Mem.other' V _ v s h) else none
+  | undir s => if h : v ∈ s then (@Mem.other' V _ v s h) else none
 
-def canGo (v : V) (e : edge V) (w : V) : Bool := w ∈ e.gofrom? v
+def canGo [DecidableEq V] (v : V) (e : edge V) (w : V) : Bool := w ∈ e.gofrom? v
 
-theorem gofrom?_iff_goback?_iff_canGo (u v : V) :
+theorem gofrom?_iff_goback?_iff_canGo [DecidableEq V] (u v : V) :
   List.TFAE [e.gofrom? u = some v, e.goback? v = some u, e.canGo u v] := by
   refine List.tfae_of_forall (e.gofrom? u = some v) _ (fun p hp => ?_)
   fin_cases hp
@@ -340,32 +343,32 @@ theorem gofrom?_iff_goback?_iff_canGo (u v : V) :
       cases a <;> simp_all [gofrom?, goback?]
       split <;> simp_all
     | undir s =>
-      simp [Sym2.eq_swap, gofrom?, goback?]
+      simp [eq_swap, gofrom?, goback?]
   · match e with
     | dir (a, b) => cases a <;> cases b <;> simp_all [canGo]
     | undir s => simp [canGo]
 
-lemma mem_startAt_of_canGo (v w : V) : e.canGo v w → v ∈ e.startAt := by
+lemma mem_startAt_of_canGo [DecidableEq V] (v w : V) : e.canGo v w → v ∈ e.startAt := by
   intro h
   match e with
   | dir (a, b) =>
     cases a <;> cases b <;> simp_all [canGo, startAt, gofrom?]
   | undir s =>
-    simp_all only [canGo, gofrom?, Option.mem_def, dite_some_none_eq_some, Sym2.exist_other'_eq,
-      decide_eq_true_eq, undir_startAt, Sym2.toMultiset_eq, Multiset.insert_eq_cons,
+    simp_all only [canGo, gofrom?, Option.mem_def, dite_some_none_eq_some, exist_other'_eq,
+      decide_eq_true_eq, undir_startAt, toMultiset_eq, Multiset.insert_eq_cons,
       Multiset.mem_cons, Multiset.mem_singleton, true_or]
 
-lemma mem_finishAt_of_canGo (v w : V) : e.canGo v w → w ∈ e.finishAt := by
+lemma mem_finishAt_of_canGo [DecidableEq V] (v w : V) : e.canGo v w → w ∈ e.finishAt := by
   intro h
   match e with
   | dir (a, b) =>
     cases a <;> cases b <;> simp_all [canGo, finishAt, gofrom?]
   | undir s =>
-    simp_all only [canGo, gofrom?, Option.mem_def, dite_some_none_eq_some, Sym2.exist_other'_eq,
-      decide_eq_true_eq, undir_finishAt, Sym2.toMultiset_eq, Multiset.insert_eq_cons,
+    simp_all only [canGo, gofrom?, Option.mem_def, dite_some_none_eq_some, exist_other'_eq,
+      decide_eq_true_eq, undir_finishAt, toMultiset_eq, Multiset.insert_eq_cons,
       Multiset.mem_cons, Multiset.mem_singleton, or_true]
 
-lemma isLoop_of_canGo_self : (∃ u, e.canGo u u) → e.isLoop := by
+lemma isLoop_of_canGo_self [DecidableEq V] : (∃ u, e.canGo u u) → e.isLoop := by
   match e with
   | dir (a, b) =>
     rintro ⟨ u, hu ⟩
@@ -373,31 +376,31 @@ lemma isLoop_of_canGo_self : (∃ u, e.canGo u u) → e.isLoop := by
     cases a <;> cases b <;> simp_all [Option.some.injEq, ite_some_none_eq_some, dir_isLoop_iff]
   | undir s =>
     rintro ⟨ u, hu ⟩
-    simp only [canGo, gofrom?, Option.mem_def, dite_some_none_eq_some, Sym2.exist_other'_eq,
+    simp only [canGo, gofrom?, Option.mem_def, dite_some_none_eq_some, exist_other'_eq,
       decide_eq_true_eq] at hu
     subst hu
-    simp only [undir_isLoop_iff, Sym2.isDiag_iff_proj_eq]
+    simp only [undir_isLoop_iff, isDiag_iff_proj_eq]
 
 
-lemma undir_gofrom?_comm (s : Sym2 V) (v w : V) :
+lemma undir_gofrom?_comm [DecidableEq V] (s : Sym2 V) (v w : V) :
     (undir s).gofrom? v = some w ↔ (undir s).gofrom? w = some v := by
-  simp only [gofrom?, dite_some_none_eq_some, Sym2.exist_other'_eq]
+  simp only [gofrom?, dite_some_none_eq_some, exist_other'_eq]
   refine Eq.congr_right ?h
-  exact Sym2.eq_swap
+  exact eq_swap
 
 @[simp]
-lemma dir_canGo (a b : V) : (dir (some a, some b)).canGo a b := by
+lemma dir_canGo [DecidableEq V] (a b : V) : (dir (some a, some b)).canGo a b := by
   simp only [canGo, gofrom?, ↓reduceIte, Option.mem_def, decide_True]
 
 @[simp]
-lemma undir_canGo (a b : V) : (undir s(a, b)).canGo a b := by
-  simp only [canGo, gofrom?, Option.mem_def, dite_some_none_eq_some, Sym2.exist_other'_eq,
+lemma undir_canGo [DecidableEq V] (a b : V) : (undir s(a, b)).canGo a b := by
+  simp only [canGo, gofrom?, Option.mem_def, dite_some_none_eq_some, exist_other'_eq,
     decide_eq_true_eq]
 
 @[simp]
-lemma undir_canGo_inf_sup [LinearOrder V] (s : Sym2 V) : (undir s).canGo s.inf s.sup := by
-  simp only [canGo, gofrom?, Option.mem_def, dite_some_none_eq_some, Sym2.exist_other'_eq,
-    Sym2.inf_sup_eq_self, decide_True]
+lemma undir_canGo_inf_sup [DecidableEq V] (s : Sym2 V) : (undir s).canGo s.out.1 s.out.2 := by
+  simp only [canGo, gofrom?, Option.mem_def, dite_some_none_eq_some, exist_other'_eq,
+    Prod.mk.eta, Quot.out_eq, decide_True]
 
 
 @[simp]
@@ -406,17 +409,17 @@ def flip : edge V := match e with
   | s => s
 
 @[simp]
-lemma flip_gofrom? : e.flip.gofrom? = e.goback? := by
+lemma flip_gofrom? [DecidableEq V] : e.flip.gofrom? = e.goback? := by
   unfold flip goback? gofrom?
   rcases e <;> simp only
 
 @[simp]
-lemma flip_goback? : e.flip.goback? = e.gofrom? := by
+lemma flip_goback? [DecidableEq V] : e.flip.goback? = e.gofrom? := by
   unfold flip goback? gofrom?
   rcases e <;> simp only
 
 @[simp]
-lemma canGo_flip (v w : V) : e.flip.canGo w v = e.canGo v w  := by
+lemma canGo_flip [DecidableEq V] (v w : V) : e.flip.canGo w v = e.canGo v w  := by
   unfold flip canGo
   match e with
   | dir (a,b) =>
@@ -453,7 +456,7 @@ lemma all_iff (P : V → Bool) : e.all P ↔ (∀ v ∈ e, P v) := by match e wi
   | undir s => simp only [all, instedgeMem, endAt, Multiset.insert_eq_cons, Multiset.empty_eq_zero,
     List.foldl_cons, Multiset.cons_zero, List.foldl_nil, mem_undir_iff, Sym2.all_iff]
 
-variable {W U : Type*} [LinearOrder W] [LinearOrder U]
+variable {W U : Type*}
 
 def map (f : V → W) : edge V → edge W
 | dir (a, b) => dir (a.map f, b.map f)
@@ -467,8 +470,8 @@ lemma mem_map_of_mem (f : V → W) (v : V) (e : edge V) : v ∈ e → f v ∈ e.
     exact h.imp (by rw [·]) (by rw [·])
   | undir s =>
     simp_all only [instedgeMem, endAt, Multiset.insert_eq_cons, Multiset.empty_eq_zero,
-      List.foldl_cons, Multiset.cons_zero, List.foldl_nil, Sym2.mem_toMultiset_iff, map,
-      Sym2.mem_map]
+      List.foldl_cons, Multiset.cons_zero, List.foldl_nil, mem_toMultiset_iff, map,
+      mem_map]
     use v
 
 lemma mem_map (f : V → W) (v : W) (e : edge V) (h : v ∈ e.map f): ∃ y ∈ e, f y = v := by
@@ -478,7 +481,7 @@ lemma mem_map (f : V → W) (v : W) (e : edge V) (h : v ∈ e.map f): ∃ y ∈ 
     rcases h with rfl | rfl <;> simp
   | undir s =>
     simp_all only [instedgeMem, endAt, Multiset.insert_eq_cons, Multiset.empty_eq_zero,
-      List.foldl_cons, Multiset.cons_zero, List.foldl_nil, map, Sym2.mem_toMultiset_iff,
+      List.foldl_cons, Multiset.cons_zero, List.foldl_nil, map, mem_toMultiset_iff,
       Sym2.mem_map]
 
 @[simp]
@@ -557,29 +560,32 @@ lemma map_eq_undir (f : V → W) (e : edge V) (s : Sym2 W) :
 
 
 @[simp]
-lemma map_startAt (f : V → W) (e : edge V) : (e.map f).startAt = e.startAt.map f := by
+lemma map_startAt [DecidableEq W] (f : V → W) (e : edge V) :
+    (e.map f).startAt = e.startAt.map f := by
   match e with
   | dir (a, b) =>
     cases a <;> cases b <;> simp_all [startAt, map, Multiset.map_cons, Multiset.map_zero]
-  | undir s => simp only [map, undir_startAt, Sym2.map_toMultiset]
+  | undir s => simp only [map, undir_startAt, map_toMultiset]
 
 @[simp]
-lemma map_finishAt (f : V → W) (e : edge V) : (e.map f).finishAt = e.finishAt.map f := by
+lemma map_finishAt [DecidableEq W] (f : V → W) (e : edge V) :
+    (e.map f).finishAt = e.finishAt.map f := by
   match e with
   | dir (a, b) =>
     cases a <;> cases b <;> simp_all [finishAt, map, Multiset.map_cons, Multiset.map_zero]
-  | undir s => simp only [map, undir_finishAt, Sym2.map_toMultiset]
+  | undir s => simp only [map, undir_finishAt, map_toMultiset]
 
 @[simp]
 lemma map_id : e.map id = e := by
-  cases e <;> simp only [map, Option.map_id_fun, id_eq, Prod.mk.eta, Sym2.map_id']
+  cases e <;> simp only [map, Option.map_id_fun, id_eq, Prod.mk.eta, map_id']
 
 @[simp]
 lemma map_comp (f : V → W) (g : W → U) (e : edge V) : e.map (g ∘ f) = (e.map f).map g := by
-  cases e <;> simp only [map, Option.map_map, Sym2.map_map]
+  cases e <;> simp only [map, Option.map_map, map_map]
 
 @[simp]
-lemma map_canGo (f : V ↪ W) (v w : V) : (e.map f).canGo (f v) (f w) ↔ e.canGo v w := by
+lemma map_canGo [DecidableEq V] [DecidableEq W] (f : V ↪ W) (v w : V) :
+    (e.map f).canGo (f v) (f w) ↔ e.canGo v w := by
   match e with
   | dir (a, b) =>
     cases a <;> cases b <;> simp_all [canGo, gofrom?, map, Option.map_none', Option.map_some',
@@ -587,16 +593,16 @@ lemma map_canGo (f : V ↪ W) (v w : V) : (e.map f).canGo (f v) (f w) ↔ e.canG
       Bool.and_eq_true, decide_eq_true_eq, and_congr_left_iff]
   | undir s =>
     simp only [canGo, gofrom?, map_undir, Option.mem_def, dite_some_none_eq_some,
-      Sym2.exist_other'_eq, decide_eq_true_eq]
+      exist_other'_eq, decide_eq_true_eq]
     constructor
     · rintro h
       ext x
-      rw [Sym2.eq_mk_out s, Sym2.map_pair_eq, Sym2.ext_iff] at h
+      rw [eq_mk_out s, map_pair_eq, Sym2.ext_iff] at h
       specialize h (f x)
-      rw [Sym2.eq_mk_out s, Sym2.mem_iff]
-      simpa only [Sym2.mem_iff, EmbeddingLike.apply_eq_iff_eq, Prod.mk.eta, Quot.out_eq] using h
+      rw [eq_mk_out s, mem_iff]
+      simpa only [mem_iff, EmbeddingLike.apply_eq_iff_eq, Prod.mk.eta, Quot.out_eq] using h
     · rintro rfl
-      simp only [Sym2.map_pair_eq]
+      simp only [map_pair_eq]
 
 
 def pmap {P : V → Prop} (f : ∀ a, P a → W) (e : edge V) : (∀ v ∈ e, P v) → edge W := by
@@ -672,7 +678,7 @@ lemma pmap_startAt {P : V → Prop} (e : edge V) (f : ∀ a, P a → W) (h : ∀
   | dir (a, b) =>
     cases a <;> cases b <;> simp_all only [pmap, Option.pmap, dir_startAt, Option.isSome_some,
       Option.get_some, Multiset.empty_eq_zero, dite_eq_ite, ite_true] <;> rfl
-  | undir s => simp only [startAt, pmap, Sym2.pmap_toMultiset]
+  | undir s => simp only [startAt, pmap, pmap_toMultiset]
 
 @[simp]
 lemma pmap_finishAt {P : V → Prop} (e : edge V) (f : ∀ a, P a → W) (h : ∀ v ∈ e, P v) :
@@ -687,20 +693,20 @@ lemma pmap_finishAt {P : V → Prop} (e : edge V) (f : ∀ a, P a → W) (h : �
 
 end edge
 
-inductive fullEdge (V : Type*) [LinearOrder V]
+inductive fullEdge (V : Type*)
 | dir : V × V → fullEdge V
 | undir : Sym2 V → fullEdge V
 
-variable {V : Type*} [LinearOrder V]
+variable {V : Type*}
 namespace fullEdge
 
-def v1 : fullEdge V → V
+noncomputable def v1 : fullEdge V → V
 | dir (a, _) => a
-| undir s => s.inf
+| undir s => s.out.1
 
-def v2 : fullEdge V → V
+noncomputable def v2 : fullEdge V → V
 | dir (_, b) => b
-| undir s => s.sup
+| undir s => s.out.2
 
 end fullEdge
 
@@ -711,8 +717,8 @@ def toFullEdge (e : edge V) (he : e.isFull) : fullEdge V :=
   | edge.dir (some a, some b), _ => fullEdge.dir (a, b)
   | edge.undir s, _ => fullEdge.undir s
 
-def v1 (e : edge V) (he : e.isFull) : V := (toFullEdge e he).v1
-def v2 (e : edge V) (he : e.isFull) : V := (toFullEdge e he).v2
+noncomputable def v1 (e : edge V) (he : e.isFull) : V := (toFullEdge e he).v1
+noncomputable def v2 (e : edge V) (he : e.isFull) : V := (toFullEdge e he).v2
 
 -- @[simp]
 -- lemma edge.toFullEdge_eq_dir (a b : V) (he : (edge.dir (some a, some b)).isFull) :
@@ -728,7 +734,7 @@ lemma dir_v1 (a b : V) (he : (dir (some a, some b)).isFull) :
 
 @[simp]
 lemma undir_v1 (s : Sym2 V) :
-  (toFullEdge (undir s) (undir_isFull s)).v1 = s.inf := rfl
+  (toFullEdge (undir s) (undir_isFull s)).v1 = s.out.1 := rfl
 
 @[simp]
 lemma dir_v2 (a b : V) (he : (dir (some a, some b)).isFull) :
@@ -736,15 +742,15 @@ lemma dir_v2 (a b : V) (he : (dir (some a, some b)).isFull) :
 
 @[simp]
 lemma undir_v2 (s : Sym2 V) :
-  (toFullEdge (undir s) (undir_isFull s)).v2 = s.sup := rfl
+  (toFullEdge (undir s) (undir_isFull s)).v2 = s.out.2 := rfl
 
 @[simp]
 lemma undir_v12_eq (s : Sym2 V) :
   undir s((toFullEdge (undir s) (undir_isFull s)).v1,
     (toFullEdge (undir s) (undir_isFull s)).v2) = undir s := by
-  simp only [undir_v1, undir_v2, Sym2.inf_sup_eq_self]
+  simp only [undir_v1, undir_v2, Prod.mk.eta, Quot.out_eq]
 
-lemma canGo_v1_v2 (e : edge V) (he : e.isFull) : canGo (e.v1 he) e (e.v2 he) := by
+lemma canGo_v1_v2 [DecidableEq V] (e : edge V) (he : e.isFull) : canGo (e.v1 he) e (e.v2 he) := by
   match e, he with
   | edge.dir (some a, some b), _ => simp only [v1, dir_v1, v2, dir_v2, dir_canGo]
   | edge.undir s, _ => simp [v1, v2]
@@ -753,7 +759,7 @@ lemma canGo_v1_v2 (e : edge V) (he : e.isFull) : canGo (e.v1 he) e (e.v2 he) := 
 lemma isLoop_iff_v1_eq_v2 (e : edge V) (he : e.isFull) : e.isLoop ↔ e.v1 he = e.v2 he := by
   match e, he with
   | edge.dir (some a, some b), _ => simp only [v1, dir_v1, v2, dir_v2, dir_isLoop_iff]
-  | edge.undir s, _ => simp only [undir_isLoop_iff, Sym2.isDiag_iff_inf_eq_sup, v1, undir_v1, v2,
+  | edge.undir s, _ => simp only [undir_isLoop_iff, isDiag_iff_out_fst_eq_out_snd, v1, undir_v1, v2,
     undir_v2]
 
 end edge
